ReverseAddNext.fst
@@ -6,6 +6,7 @@ open ReverseAdd
 open ReverseAddCarry
 open ReverseAddWitness
 open ReverseAddOverflowProfile
+open FStar.Classical
 open FStar.List.Tot
 
 let next_source : numeral 10 =
@@ -239,4 +240,320 @@ let local_profile_witness_947154635293536341848 () : Lemma (
   assert (trace_sum_at next_source 0 == 8);
   reverse_add_177104867844767940077_to_947154635293536341848 ();
   no_overflow_outer_sum_6_to_9_implies_next_witness next_source;
+  ()
+
+let next2_source : numeral 10 = next_target
+
+let next2_reversed : numeral 10 =
+  [9; 4; 7; 1; 5; 4; 6; 3; 5; 2; 9; 3; 5; 3; 6; 3; 4; 1; 8; 4; 8]
+
+let next2_target : numeral 10 =
+  [7; 9; 5; 3; 9; 7; 2; 7; 0; 6; 8; 6; 0; 7; 2; 8; 9; 2; 5; 9; 7; 1]
+
+let reverse_list_next2_source () : Lemma (rev next2_source == next2_reversed) =
+  assert (rev [9] == [9]);
+  rev_cons 4 [9];
+  rev_cons 7 [4; 9];
+  rev_cons 1 [7; 4; 9];
+  rev_cons 8 [1; 7; 4; 9];
+  rev_cons 4 [8; 1; 7; 4; 9];
+  rev_cons 3 [4; 8; 1; 7; 4; 9];
+  rev_cons 6 [3; 4; 8; 1; 7; 4; 9];
+  rev_cons 3 [6; 3; 4; 8; 1; 7; 4; 9];
+  rev_cons 5 [3; 6; 3; 4; 8; 1; 7; 4; 9];
+  rev_cons 3 [5; 3; 6; 3; 4; 8; 1; 7; 4; 9];
+  rev_cons 9 [3; 5; 3; 6; 3; 4; 8; 1; 7; 4; 9];
+  rev_cons 2 [9; 3; 5; 3; 6; 3; 4; 8; 1; 7; 4; 9];
+  rev_cons 5 [2; 9; 3; 5; 3; 6; 3; 4; 8; 1; 7; 4; 9];
+  rev_cons 3 [5; 2; 9; 3; 5; 3; 6; 3; 4; 8; 1; 7; 4; 9];
+  rev_cons 6 [3; 5; 2; 9; 3; 5; 3; 6; 3; 4; 8; 1; 7; 4; 9];
+  rev_cons 4 [6; 3; 5; 2; 9; 3; 5; 3; 6; 3; 4; 8; 1; 7; 4; 9];
+  rev_cons 5 [4; 6; 3; 5; 2; 9; 3; 5; 3; 6; 3; 4; 8; 1; 7; 4; 9];
+  rev_cons 1 [5; 4; 6; 3; 5; 2; 9; 3; 5; 3; 6; 3; 4; 8; 1; 7; 4; 9];
+  rev_cons 4 [1; 5; 4; 6; 3; 5; 2; 9; 3; 5; 3; 6; 3; 4; 8; 1; 7; 4; 9];
+  rev_cons 8 [4; 1; 5; 4; 6; 3; 5; 2; 9; 3; 5; 3; 6; 3; 4; 8; 1; 7; 4; 9];
+  ()
+
+let value_next2_reversed () : Lemma (
+    value next2_reversed == 848143635392536451749) =
+  value_cons #10 9 [4; 7; 1; 5; 4; 6; 3; 5; 2; 9; 3; 5; 3; 6; 3; 4; 1; 8; 4; 8];
+  value_cons #10 4 [7; 1; 5; 4; 6; 3; 5; 2; 9; 3; 5; 3; 6; 3; 4; 1; 8; 4; 8];
+  value_cons #10 7 [1; 5; 4; 6; 3; 5; 2; 9; 3; 5; 3; 6; 3; 4; 1; 8; 4; 8];
+  value_cons #10 1 [5; 4; 6; 3; 5; 2; 9; 3; 5; 3; 6; 3; 4; 1; 8; 4; 8];
+  value_cons #10 5 [4; 6; 3; 5; 2; 9; 3; 5; 3; 6; 3; 4; 1; 8; 4; 8];
+  value_cons #10 4 [6; 3; 5; 2; 9; 3; 5; 3; 6; 3; 4; 1; 8; 4; 8];
+  value_cons #10 6 [3; 5; 2; 9; 3; 5; 3; 6; 3; 4; 1; 8; 4; 8];
+  value_cons #10 3 [5; 2; 9; 3; 5; 3; 6; 3; 4; 1; 8; 4; 8];
+  value_cons #10 5 [2; 9; 3; 5; 3; 6; 3; 4; 1; 8; 4; 8];
+  value_cons #10 2 [9; 3; 5; 3; 6; 3; 4; 1; 8; 4; 8];
+  value_cons #10 9 [3; 5; 3; 6; 3; 4; 1; 8; 4; 8];
+  value_cons #10 3 [5; 3; 6; 3; 4; 1; 8; 4; 8];
+  value_cons #10 5 [3; 6; 3; 4; 1; 8; 4; 8];
+  value_cons #10 3 [6; 3; 4; 1; 8; 4; 8];
+  value_cons #10 6 [3; 4; 1; 8; 4; 8];
+  value_cons #10 3 [4; 1; 8; 4; 8];
+  value_cons #10 4 [1; 8; 4; 8];
+  value_cons #10 1 [8; 4; 8];
+  value_cons #10 8 [4; 8];
+  value_cons #10 4 [8];
+  value_cons #10 8 [];
+  ()
+
+let value_next2_target () : Lemma (
+    value next2_target == 1795298270686072793597) =
+  value_cons #10 7 [9; 5; 3; 9; 7; 2; 7; 0; 6; 8; 6; 0; 7; 2; 8; 9; 2; 5; 9; 7; 1];
+  value_cons #10 9 [5; 3; 9; 7; 2; 7; 0; 6; 8; 6; 0; 7; 2; 8; 9; 2; 5; 9; 7; 1];
+  value_cons #10 5 [3; 9; 7; 2; 7; 0; 6; 8; 6; 0; 7; 2; 8; 9; 2; 5; 9; 7; 1];
+  value_cons #10 3 [9; 7; 2; 7; 0; 6; 8; 6; 0; 7; 2; 8; 9; 2; 5; 9; 7; 1];
+  value_cons #10 9 [7; 2; 7; 0; 6; 8; 6; 0; 7; 2; 8; 9; 2; 5; 9; 7; 1];
+  value_cons #10 7 [2; 7; 0; 6; 8; 6; 0; 7; 2; 8; 9; 2; 5; 9; 7; 1];
+  value_cons #10 2 [7; 0; 6; 8; 6; 0; 7; 2; 8; 9; 2; 5; 9; 7; 1];
+  value_cons #10 7 [0; 6; 8; 6; 0; 7; 2; 8; 9; 2; 5; 9; 7; 1];
+  value_cons #10 0 [6; 8; 6; 0; 7; 2; 8; 9; 2; 5; 9; 7; 1];
+  value_cons #10 6 [8; 6; 0; 7; 2; 8; 9; 2; 5; 9; 7; 1];
+  value_cons #10 8 [6; 0; 7; 2; 8; 9; 2; 5; 9; 7; 1];
+  value_cons #10 6 [0; 7; 2; 8; 9; 2; 5; 9; 7; 1];
+  value_cons #10 0 [7; 2; 8; 9; 2; 5; 9; 7; 1];
+  value_cons #10 7 [2; 8; 9; 2; 5; 9; 7; 1];
+  value_cons #10 2 [8; 9; 2; 5; 9; 7; 1];
+  value_cons #10 8 [9; 2; 5; 9; 7; 1];
+  value_cons #10 9 [2; 5; 9; 7; 1];
+  value_cons #10 2 [5; 9; 7; 1];
+  value_cons #10 5 [9; 7; 1];
+  value_cons #10 9 [7; 1];
+  value_cons #10 7 [1];
+  value_cons #10 1 [];
+  ()
+
+let canonical_next2_reversed () : Lemma (canonical #10 next2_reversed) =
+  assert (canonical #10 [8]);
+  canonical_cons #10 4 [8];
+  canonical_cons #10 1 [4; 8];
+  canonical_cons #10 3 [1; 4; 8];
+  canonical_cons #10 6 [3; 1; 4; 8];
+  canonical_cons #10 3 [6; 3; 1; 4; 8];
+  canonical_cons #10 5 [3; 6; 3; 1; 4; 8];
+  canonical_cons #10 3 [5; 3; 6; 3; 1; 4; 8];
+  canonical_cons #10 9 [3; 5; 3; 6; 3; 1; 4; 8];
+  canonical_cons #10 2 [9; 3; 5; 3; 6; 3; 1; 4; 8];
+  canonical_cons #10 5 [2; 9; 3; 5; 3; 6; 3; 1; 4; 8];
+  canonical_cons #10 3 [5; 2; 9; 3; 5; 3; 6; 3; 1; 4; 8];
+  canonical_cons #10 5 [3; 5; 2; 9; 3; 5; 3; 6; 3; 1; 4; 8];
+  canonical_cons #10 3 [5; 3; 5; 2; 9; 3; 5; 3; 6; 3; 1; 4; 8];
+  canonical_cons #10 6 [3; 5; 3; 5; 2; 9; 3; 5; 3; 6; 3; 1; 4; 8];
+  canonical_cons #10 4 [6; 3; 5; 3; 5; 2; 9; 3; 5; 3; 6; 3; 1; 4; 8];
+  canonical_cons #10 5 [4; 6; 3; 5; 3; 5; 2; 9; 3; 5; 3; 6; 3; 1; 4; 8];
+  canonical_cons #10 1 [5; 4; 6; 3; 5; 3; 5; 2; 9; 3; 5; 3; 6; 3; 1; 4; 8];
+  canonical_cons #10 7 [1; 5; 4; 6; 3; 5; 3; 5; 2; 9; 3; 5; 3; 6; 3; 1; 4; 8];
+  canonical_cons #10 4 [7; 1; 5; 4; 6; 3; 5; 3; 5; 2; 9; 3; 5; 3; 6; 3; 1; 4; 8];
+  canonical_cons #10 9 [4; 7; 1; 5; 4; 6; 3; 5; 3; 5; 2; 9; 3; 5; 3; 6; 3; 1; 4; 8];
+  ()
+
+let canonical_next2_target () : Lemma (canonical #10 next2_target) =
+  assert (canonical #10 [1]);
+  canonical_cons #10 7 [1];
+  canonical_cons #10 9 [7; 1];
+  canonical_cons #10 5 [9; 7; 1];
+  canonical_cons #10 2 [5; 9; 7; 1];
+  canonical_cons #10 9 [2; 5; 9; 7; 1];
+  canonical_cons #10 8 [9; 2; 5; 9; 7; 1];
+  canonical_cons #10 2 [8; 9; 2; 5; 9; 7; 1];
+  canonical_cons #10 7 [2; 8; 9; 2; 5; 9; 7; 1];
+  canonical_cons #10 0 [7; 2; 8; 9; 2; 5; 9; 7; 1];
+  canonical_cons #10 6 [0; 7; 2; 8; 9; 2; 5; 9; 7; 1];
+  canonical_cons #10 8 [6; 0; 7; 2; 8; 9; 2; 5; 9; 7; 1];
+  canonical_cons #10 6 [8; 6; 0; 7; 2; 8; 9; 2; 5; 9; 7; 1];
+  canonical_cons #10 0 [6; 8; 6; 0; 7; 2; 8; 9; 2; 5; 9; 7; 1];
+  canonical_cons #10 7 [0; 6; 8; 6; 0; 7; 2; 8; 9; 2; 5; 9; 7; 1];
+  canonical_cons #10 2 [7; 0; 6; 8; 6; 0; 7; 2; 8; 9; 2; 5; 9; 7; 1];
+  canonical_cons #10 7 [2; 7; 0; 6; 8; 6; 0; 7; 2; 8; 9; 2; 5; 9; 7; 1];
+  canonical_cons #10 3 [7; 2; 7; 0; 6; 8; 6; 0; 7; 2; 8; 9; 2; 5; 9; 7; 1];
+  canonical_cons #10 5 [3; 7; 2; 7; 0; 6; 8; 6; 0; 7; 2; 8; 9; 2; 5; 9; 7; 1];
+  canonical_cons #10 9 [5; 3; 7; 2; 7; 0; 6; 8; 6; 0; 7; 2; 8; 9; 2; 5; 9; 7; 1];
+  canonical_cons #10 7 [9; 5; 3; 7; 2; 7; 0; 6; 8; 6; 0; 7; 2; 8; 9; 2; 5; 9; 7; 1];
+  canonical_cons #10 9 [7; 9; 5; 3; 7; 2; 7; 0; 6; 8; 6; 0; 7; 2; 8; 9; 2; 5; 9; 7; 1];
+  canonical_cons #10 7 [9; 7; 9; 5; 3; 7; 2; 7; 0; 6; 8; 6; 0; 7; 2; 8; 9; 2; 5; 9; 7; 1];
+  ()
+
+let reverse_digits_next2_source () : Lemma (
+    reverse_digits #10 next2_source == next2_reversed) =
+  ReverseAddNext.canonical_next_target ();
+  reverse_list_next2_source ();
+  value_next2_reversed ();
+  canonical_next2_reversed ();
+  reverse_digits_canonical #10 next2_source;
+  normalize_value #10 (rev next2_source);
+  assert (value (reverse_digits #10 next2_source) ==
+    848143635392536451749);
+  digits_of_nat_of_canonical #10 (reverse_digits #10 next2_source);
+  digits_of_nat_of_canonical #10 next2_reversed;
+  assert (reverse_digits #10 next2_source == next2_reversed);
+  ()
+
+let reverse_add_947154635293536341848_to_1795298270686072793597 () : Lemma (
+    reverse_add #10 next2_source == next2_target) =
+  ReverseAddNext.canonical_next_target ();
+  reverse_add_value #10 next2_source;
+  ReverseAddNext.value_next_target ();
+  reverse_digits_next2_source ();
+  value_next2_reversed ();
+  value_next2_target ();
+  assert (value (reverse_add #10 next2_source) ==
+    1795298270686072793597);
+  reverse_add_canonical #10 next2_source;
+  digits_of_nat_of_canonical #10 (reverse_add #10 next2_source);
+  canonical_next2_target ();
+  digits_of_nat_of_canonical #10 next2_target;
+  assert (reverse_add #10 next2_source == next2_target);
+  ()
+
+let trace_digits_profile_947154635293536341848 () : Lemma (
+    trace_digits next2_source == next2_target) =
+  reverse_add_947154635293536341848_to_1795298270686072793597 ();
+  trace_digits_equals_reverse_add next2_source;
+  assert (trace_digits next2_source == next2_target);
+  ()
+
+let trace_carries_next2_source () : Lemma (trace_carries next2_source ==
+    [0; 1; 0; 1; 0; 0; 0; 1; 0; 1; 0; 1; 0; 1; 0; 1; 0; 0; 0; 1; 0; 1]) =
+  reverse_list_next2_source ();
+  assert (trace_carries next2_source ==
+    (add_trace #10 next2_source next2_reversed 0).carries);
+  add_trace_carries_step #10 8 9
+    [4; 8; 1; 4; 3; 6; 3; 5; 3; 9; 2; 5; 3; 6; 4; 5; 1; 7; 4; 9]
+    [4; 7; 1; 5; 4; 6; 3; 5; 2; 9; 3; 5; 3; 6; 3; 4; 1; 8; 4; 8] 0;
+  add_trace_carries_step #10 4 4
+    [8; 1; 4; 3; 6; 3; 5; 3; 9; 2; 5; 3; 6; 4; 5; 1; 7; 4; 9]
+    [7; 1; 5; 4; 6; 3; 5; 2; 9; 3; 5; 3; 6; 3; 4; 1; 8; 4; 8] 1;
+  add_trace_carries_step #10 8 7
+    [1; 4; 3; 6; 3; 5; 3; 9; 2; 5; 3; 6; 4; 5; 1; 7; 4; 9]
+    [1; 5; 4; 6; 3; 5; 2; 9; 3; 5; 3; 6; 3; 4; 1; 8; 4; 8] 0;
+  add_trace_carries_step #10 1 1
+    [4; 3; 6; 3; 5; 3; 9; 2; 5; 3; 6; 4; 5; 1; 7; 4; 9]
+    [5; 4; 6; 3; 5; 2; 9; 3; 5; 3; 6; 3; 4; 1; 8; 4; 8] 1;
+  add_trace_carries_step #10 4 5
+    [3; 6; 3; 5; 3; 9; 2; 5; 3; 6; 4; 5; 1; 7; 4; 9]
+    [4; 6; 3; 5; 2; 9; 3; 5; 3; 6; 3; 4; 1; 8; 4; 8] 0;
+  add_trace_carries_step #10 3 4
+    [6; 3; 5; 3; 9; 2; 5; 3; 6; 4; 5; 1; 7; 4; 9]
+    [6; 3; 5; 2; 9; 3; 5; 3; 6; 3; 4; 1; 8; 4; 8] 0;
+  add_trace_carries_step #10 6 6
+    [3; 5; 3; 9; 2; 5; 3; 6; 4; 5; 1; 7; 4; 9]
+    [3; 5; 2; 9; 3; 5; 3; 6; 3; 4; 1; 8; 4; 8] 0;
+  add_trace_carries_step #10 3 3
+    [5; 3; 9; 2; 5; 3; 6; 4; 5; 1; 7; 4; 9]
+    [5; 2; 9; 3; 5; 3; 6; 3; 4; 1; 8; 4; 8] 1;
+  add_trace_carries_step #10 5 5
+    [3; 9; 2; 5; 3; 6; 4; 5; 1; 7; 4; 9]
+    [2; 9; 3; 5; 3; 6; 3; 4; 1; 8; 4; 8] 0;
+  add_trace_carries_step #10 3 2
+    [9; 2; 5; 3; 6; 4; 5; 1; 7; 4; 9]
+    [9; 3; 5; 3; 6; 3; 4; 1; 8; 4; 8] 1;
+  add_trace_carries_step #10 9 9
+    [2; 5; 3; 6; 4; 5; 1; 7; 4; 9]
+    [3; 5; 3; 6; 3; 4; 1; 8; 4; 8] 0;
+  add_trace_carries_step #10 2 3
+    [5; 3; 6; 4; 5; 1; 7; 4; 9]
+    [5; 3; 6; 3; 4; 1; 8; 4; 8] 1;
+  add_trace_carries_step #10 5 5
+    [3; 6; 4; 5; 1; 7; 4; 9]
+    [3; 6; 3; 4; 1; 8; 4; 8] 0;
+  add_trace_carries_step #10 3 3
+    [6; 4; 5; 1; 7; 4; 9]
+    [6; 3; 4; 1; 8; 4; 8] 1;
+  add_trace_carries_step #10 6 6
+    [4; 5; 1; 7; 4; 9]
+    [3; 4; 1; 8; 4; 8] 0;
+  add_trace_carries_step #10 4 3
+    [5; 1; 7; 4; 9]
+    [4; 1; 8; 4; 8] 1;
+  add_trace_carries_step #10 5 4
+    [1; 7; 4; 9]
+    [1; 8; 4; 8] 0;
+  add_trace_carries_step #10 1 1
+    [7; 4; 9]
+    [8; 4; 8] 0;
+  add_trace_carries_step #10 7 8
+    [4; 9]
+    [4; 8] 0;
+  add_trace_carries_step #10 4 4
+    [9]
+    [8] 1;
+  add_trace_carries_step #10 9 8 [] [] 0;
+  assert ((add_trace #10 [] [] 1).carries == [1]);
+  assert ((add_trace #10 next2_source next2_reversed 0).carries ==
+    [0; 1; 0; 1; 0; 0; 0; 1; 0; 1; 0; 1; 0; 1; 0; 1; 0; 0; 0; 1; 0; 1]);
+  ()
+
+let trace_profile_shape_947154635293536341848 () : Lemma (
+    length (trace_digits next2_source) == length next2_source + 1) =
+  trace_digits_profile_947154635293536341848 ();
+  length_of_eq #(digit 10) (trace_digits next2_source) next2_target;
+  assert (length next2_target == length next2_source + 1);
+  ()
+
+let trace_profile_final_carry_947154635293536341848 () : Lemma (
+    nth (trace_carries next2_source) (length next2_source) == Some 1) =
+  trace_profile_shape_947154635293536341848 ();
+  ReverseAddContinuation.final_carry_from_overflow_length next2_source;
+  ()
+
+let trace_profile_sums_947154635293536341848 () : Lemma (
+    trace_sum_at next2_source 0 == 17 /\
+    trace_sum_at next2_source 1 == 8 /\
+    trace_sum_at next2_source 20 == 17) =
+  reverse_list_next2_source ();
+  ()
+
+let trace_profile_carry_facts_947154635293536341848 () : Lemma (
+    trace_carry_at next2_source 1 == 1 /\
+    trace_carry_at next2_source 20 == 0 /\
+    trace_carry_at next2_source 2 == 0 /\
+    trace_carry_at next2_source 21 == 1) =
+  trace_carries_next2_source ();
+  ()
+
+let overflow_precondition_1795298270686072793597 () : Lemma (
+    canonical #10 next2_source /\
+    next2_source <> [] /\
+    length (trace_digits next2_source) == length next2_source + 1 /\
+    nth (trace_carries next2_source) (length next2_source) == Some 1 /\
+    1 <= trace_sum_at next2_source 0 /\
+    trace_sum_at next2_source 0 <= 18 /\
+    trace_sum_at next2_source 0 <> 10 /\
+    exists (i:nat). 0 < i /\ i < length next2_source /\
+      trace_sum_at next2_source i +
+          trace_sum_at next2_source (length next2_source - i) +
+          trace_carry_at next2_source i +
+          trace_carry_at next2_source (length next2_source - i) >=
+        10 + 10 *
+          (trace_carry_at next2_source (i + 1) +
+           trace_carry_at next2_source (length next2_source - i + 1))) =
+  ReverseAddNext.canonical_next_target ();
+  assert (next2_source <> []);
+  trace_profile_shape_947154635293536341848 ();
+  trace_profile_final_carry_947154635293536341848 ();
+  trace_profile_sums_947154635293536341848 ();
+  trace_profile_carry_facts_947154635293536341848 ();
+  assert (1 <= trace_sum_at next2_source 0 /\
+    trace_sum_at next2_source 0 <= 18);
+  assert (trace_sum_at next2_source 0 <> 10);
+  let n : nat = length next2_source in
+  exists_intro
+    (fun (i:nat) -> 0 < i /\ i < n /\
+      trace_sum_at next2_source i +
+          trace_sum_at next2_source (n - i) +
+          trace_carry_at next2_source i +
+          trace_carry_at next2_source (n - i) >=
+        10 + 10 *
+          (trace_carry_at next2_source (i + 1) +
+           trace_carry_at next2_source (n - i + 1)))
+    1;
+  ()
+
+let local_profile_witness_1795298270686072793597 () : Lemma (
+    trace_local_profile_complement_witness next2_target) =
+  overflow_precondition_1795298270686072793597 ();
+  reverse_add_947154635293536341848_to_1795298270686072793597 ();
+  overflow_internal_cell_implies_next_witness next2_source;
   ()
